WIP

quotation/theories/CommonUtils.v
@@ -1,10 +1,11 @@
-From MetaCoq.Utils Require Import utils MCList.
+From MetaCoq.Utils Require Import utils monad_utils MCList.
 From MetaCoq.Common Require Import Kernames.
 From MetaCoq.Template Require MonadBasicAst MonadAst TemplateMonad Ast Loader.
 Require Import Equations.Prop.Classes.
 Require Import Coq.Lists.List.
 Import ListNotations.
 
+Local Unset Universe Minimization ToSet.
 Local Set Primitive Projections.
 Local Open Scope bs.
 Import MCMonadNotation.
@@ -69,6 +70,46 @@ Proof. cbv [b_of_dec]; destruct H; auto; discriminate. Defined.
 Definition neg_pb_of_dec {P:Prop} {H} : ~P -> @b_of_dec P H = false.
 Proof. cbv [b_of_dec]; destruct H; tauto. Defined.
 
+(* TODO: move? *)
+Definition kername_of_global_reference (g : global_reference) : option kername
+  := match g with
+     | VarRef _ => None
+     | ConstRef x => Some x
+     | IndRef ind
+     | ConstructRef ind _
+       => Some ind.(inductive_mind)
+     end.
+
+Definition replace_inductive_kn (t : inductive) (ind : inductive) : inductive
+  := {| inductive_mind := ind.(inductive_mind) ; inductive_ind := t.(inductive_ind) |}.
+
+Definition replace_inductive_modpath (mp : modpath) (ind : inductive) : inductive
+  := {| inductive_mind := (mp, snd ind.(inductive_mind)) ; inductive_ind := ind.(inductive_ind) |}.
+
+Definition rebase_global_reference (mp : modpath) (g : global_reference) : global_reference
+  := match g with
+     | VarRef x => VarRef x
+     | ConstRef (_, i) => ConstRef (mp, i)
+     | IndRef ind => IndRef (replace_inductive_modpath mp ind)
+     | ConstructRef ind idx => ConstructRef (replace_inductive_modpath mp ind) idx
+     end.
+
+(* hack around https://github.com/MetaCoq/metacoq/issues/850 *)
+Fixpoint dedup_grefs' (g : list global_reference) (seen : KernameSet.t) : list global_reference
+  := match g with
+     | nil => nil
+     | g :: gs
+       => match kername_of_global_reference g with
+          | None => g :: dedup_grefs' gs seen
+          | Some kn
+            => if KernameSet.mem kn seen
+               then dedup_grefs' gs seen
+               else g :: dedup_grefs' gs (KernameSet.add kn seen)
+          end
+     end.
+Definition dedup_grefs (g : list global_reference) : list global_reference
+  := dedup_grefs' g KernameSet.empty.
+
 Module WithTemplate.
   Import MetaCoq.Template.Loader.
   Import MetaCoq.Template.Ast.
@@ -88,6 +129,94 @@ Module WithTemplate.
             end;;
        tmUnquoteTyped A v.
   Notation transparentify v := (match tmUnfoldQed v return _ with v' => ltac:(run_template_program v' (fun v' => exact v')) end) (only parsing).
-End WithTemplate.
 
-Notation transparentify v := (WithTemplate.transparentify v) (only parsing).
+  #[local]
+    Fixpoint tmRelaxSorts (U : Universe.t -> term) (t : term) {struct t} : term
+    := match t with
+       | tRel _
+       | tVar _
+       | tInt _
+       | tFloat _
+       | tConst _ _
+       | tInd _ _
+       | tConstruct _ _ _
+         => t
+       | tEvar ev args
+         => tEvar ev (List.map (tmRelaxSorts U) args)
+       | tCast t kind v
+         => tCast (tmRelaxSorts U t) kind (tmRelaxSorts U v)
+       | tProd na ty body
+         => tProd na (tmRelaxSorts U ty) (tmRelaxSorts U body)
+       | tLambda na ty body
+         => tLambda na (tmRelaxSorts U ty) (tmRelaxSorts U body)
+       | tLetIn na def def_ty body
+         => tLetIn na (tmRelaxSorts U def) (tmRelaxSorts U def_ty) (tmRelaxSorts U body)
+       | tApp f args
+         => tApp (tmRelaxSorts U f) (List.map (tmRelaxSorts U) args)
+       | tCase ci type_info discr branches
+         => tCase ci (map_predicate (fun x => x) (tmRelaxSorts U) (tmRelaxSorts U) type_info) (tmRelaxSorts U discr) (map_branches (tmRelaxSorts U) branches)
+       | tProj proj t
+         => tProj proj (tmRelaxSorts U t)
+       | tFix mfix idx
+         => tFix (List.map (map_def (tmRelaxSorts U) (tmRelaxSorts U)) mfix) idx
+       | tCoFix mfix idx
+         => tCoFix (List.map (map_def (tmRelaxSorts U) (tmRelaxSorts U)) mfix) idx
+       | tSort s => U s
+       end.
+
+  #[local]
+    Definition tmRelaxSet (U : term) (t : term) : term
+    := tmRelaxSorts (fun s => match option_map Level.is_set (Universe.get_is_level s) with
+                              | Some true => U
+                              | _ => tSort s
+                              end)
+         t.
+
+  #[local]
+    Definition tmRelaxType (U : term) (t : term) : term
+    := tmRelaxSorts (fun s => match Universe.get_is_level s with
+                              | Some _ => U
+                              | _ => tSort s
+                              end)
+         t.
+
+  Polymorphic Definition tmRetypeRelaxSet@{U a t u} {A : Type@{a}} (x : A) : TemplateMonad@{t u} A
+    := qx <- tmQuote x;;
+       qU <- tmQuoteUniverse@{U _ _};;
+       let qx := tmRelaxSet (tSort qU) qx in
+       tmUnquoteTyped A qx.
+
+  Polymorphic Definition tmRetypeRelaxType@{U a t u} {A : Type@{a}} (x : A) : TemplateMonad@{t u} A
+    := qx <- tmQuote x;;
+       qU <- tmQuoteUniverse@{U _ _};;
+       let qx := tmRelaxType (tSort qU) qx in
+       tmUnquoteTyped A qx.
+
+  Polymorphic Definition tmQuoteToGlobalReference {A} (n : A) : TemplateMonad global_reference
+    := qn <- tmQuote n;;
+       match qn with
+       | tVar id => tmReturn (VarRef id)
+       | tConst c u => tmReturn (ConstRef c)
+       | tInd ind u => tmReturn (IndRef ind)
+       | tConstruct ind idx u => tmReturn (ConstructRef ind idx)
+       | _ => _ <- tmMsg "tmQuoteToGlobalReference: Not a global reference";;
+              _ <- tmPrint n;;
+              _ <- tmPrint qn;;
+              tmFail "tmQuoteToGlobalReference: Not a global reference"
+       end.
+
+  Polymorphic Definition tmObj_magic {A B} (x : A) : TemplateMonad B
+    := qx <- tmQuote x;;
+       tmUnquoteTyped B qx.
+
+  Polymorphic Definition tmRetype {A} (x : A) : TemplateMonad A
+    := tmObj_magic x.
+
+  Polymorphic Definition tmExtractBaseModPathFromMod (mp : qualid) : TemplateMonad modpath
+    := vs <- tmQuoteModule mp;;
+       match option_map kername_of_global_reference (hd_error vs) with
+       | Some (Some (mp, _)) => ret mp
+       | _ => tmFail "tmExtractBaseModPathFromMod: module has no accessible constant with a kername"
+       end.
+End WithTemplate.
+Export WithTemplate (transparentify, tmRetypeRelaxSet, tmRetypeRelaxType, tmQuoteToGlobalReference, tmObj_magic, tmRetype, tmExtractBaseModPathFromMod).
