quotation/theories/ToTemplate/Common/Kernames.v
@@ -1,8 +1,16 @@
+From Coq Require Import Lists.List.
 From MetaCoq.Quotation.ToTemplate Require Export Init.
 From MetaCoq.Quotation.ToTemplate Require Export (hints) Coq.Init Coq.Structures Coq.MSets Coq.FSets bytestring.
 From MetaCoq.Common Require Import Kernames.
+From MetaCoq.Utils Require Import bytestring monad_utils.
+From MetaCoq.Template Require Import Loader TemplateMonad.
+
+Local Open Scope bs.
+Import MCMonadNotation.
+Import ListNotations.
 
 #[export] Instance quote_modpath : ground_quotable modpath := ltac:(induction 1; exact _).
+
 From MetaCoq.Utils Require Export bytestring.
 From MetaCoq.Utils Require Import utils MCList.
 From MetaCoq.Template Require Import MonadBasicAst MonadAst TemplateMonad Ast Loader.
@@ -15,34 +23,161 @@ Local Set Primitive Projections.
 Local Open Scope bs.
 Import MCMonadNotation.
 
+Print relevance.
+Print mutual_inductive_body.
+Definition tmMakeQuotationOfConstants {debug:debug_opt} (do_existing_instance : bool) (cs : list global_reference) : TemplateMonad unit
+  := let warn_bad_ctx c ctx :=
+       (_ <- tmMsg "tmMakeQuotationOfModule: cannot handle polymorphism";;
+        _ <- tmPrint c;;
+        _ <- tmPrint ctx;;
+        tmReturn tt) in
+     let tmDebugMsg s := (if debug
+                          then tmMsg s
+                          else tmReturn tt) in
+     let tmDebugPrint {T} (v : T) := (if debug
+                                      then tmPrint v
+                                      else tmReturn tt) in
+     let on_bad_relevance r :=
+       (_ <- tmDebugMsg "skipping irrelevant constant";;
+        _ <- tmDebugPrint r;;
+        tmReturn []) in
+     let cs := dedup_grefs cs in
+     cs <- tmEval cbv cs;;
+     _ <- tmDebugMsg "tmMakeQuotationOfConstants: looking up module constants";;
+     ps <- monad_map
+             (fun r
+              => _ <- tmDebugMsg "tmMakeQuotationOfConstants: handling";;
+                 _ <- tmDebugPrint r;;
+                 match r with
+                 | ConstRef ((mp, name) as c)
+                   => '(inst, rel) <- (cb <- tmQuoteConstant c false;;
+                                       inst <- match cb.(cst_universes) with
+                                               | Monomorphic_ctx => tmReturn []
+                                               | (Polymorphic_ctx (univs, constraints)) as ctx
+                                                 => _ <- warn_bad_ctx r ctx;;
+                                                    tmReturn []
+                                               end;;
+                                       tmReturn (inst, cb.(cst_relevance)));;
+                      match rel with
+                      | Irrelevant => on_bad_relevance r
+                      | Relevant
+                        => let c := tConst c inst in
+                           _ <- tmDebugMsg "tmMakeQuotationOfConstants: tmUnquote";;
+                           '{| my_projT1 := cty ; my_projT2 := cv |} <- tmUnquote c;;
+                           _ <- tmDebugMsg "tmMakeQuotationOfConstants: tmUnquote done";;
+                           let ty := @quotation_of cty cv in
+                           tmReturn [("q" ++ name, {| my_projT1 := ty ; my_projT2 := c |})]
+                      end
+                 | IndRef ind
+                   => inst <- (mib <- tmQuoteInductive ind.(inductive_mind);;
+                               match mib.(ind_universes) with
+                               | Monomorphic_ctx => tmReturn []
+                               | (Polymorphic_ctx (univs, constraints)) as ctx
+                                 => _ <- warn_bad_ctx r ctx;;
+                                    tmReturn []
+                               end);;
+                      let '(mp, name) := ind.(inductive_mind) in
+                      let c := tInd ind inst in
+                      _ <- tmDebugMsg "tmMakeQuotationOfConstants: tmUnquote";;
+                      '{| my_projT1 := cty ; my_projT2 := cv |} <- tmUnquote c;;
+                      _ <- tmDebugMsg "tmMakeQuotationOfConstants: tmUnquote done";;
+                      let ty := inductive_quotation_of cv in
+                      let v : ty := {| qinductive := ind ; qinst := inst |} in
+                      tmReturn [("q" ++ name, {| my_projT1 := ty ; my_projT2 := v |})]
+                 | ConstructRef _ _ | VarRef _ => tmReturn []
+                 end)
+             cs;;
+     let ps := flat_map (fun x => x) ps in
+     _ <- tmDebugMsg "tmMakeQuotationOfConstants: relaxing Set and retyping module constants";;
+     ps <- monad_map
+             (fun '(name, {| my_projT1 := ty ; my_projT2 := v |})
+              => _ <- tmDebugMsg ("tmMakeQuotationOfConstants: relaxing " ++ name);;
+                 _ <- tmDebugPrint ("before"%bs, v, ":"%bs, ty);;
+                 ty <- tmRetypeRelaxType ty;;
+                 (* hack around https://github.com/MetaCoq/metacoq/issues/853 *)
+                 v <- tmRetypeRelaxType v;;
+                 v <- tmObj_magic v;;
+                 _ <- tmDebugPrint ("after"%bs, v, ":"%bs, ty);;
+                 tmReturn (name, {| my_projT1 := ty ; my_projT2 := v |}))
+             ps;;
+     _ <- tmDebugMsg "tmMakeQuotationOfConstants: defining module constants";;
+     ps <- monad_map
+             (fun '(name, {| my_projT1 := ty ; my_projT2 := v |})
+              => (* debugging sanity checks for hack around https://github.com/MetaCoq/metacoq/issues/853 *)
+                _ <- tmDebugPrint (tmRetype ty);;
+                _ <- tmRetype ty;;
+                _ <- tmDebugPrint (tmRetype v);;
+                _ <- tmRetype v;;
+                _ <- tmDebugPrint (@tmDefinition name ty v);;
+                n <- @tmDefinition name ty v;;
+                _ <- tmDebugMsg "tmMakeQuotationOfConstants: tmQuoteToGlobalReference";;
+                qn <- tmQuoteToGlobalReference n;;
+                tmReturn qn)
+             ps;;
+     _ <- (if do_existing_instance
+           then
+             _ <- tmDebugMsg "tmMakeQuotationOfConstants: making instances";;
+             monad_map tmExistingInstance ps
+           else tmReturn []);;
+     tmReturn tt.
+
+Definition tmMakeQuotationOfModule {debug:debug_opt} (do_existing_instance : bool) (m : qualid) : TemplateMonad _
+  := cs <- tmQuoteModule m;;
+     tmMakeQuotationOfConstants do_existing_instance cs.
+Global Arguments tmMakeQuotationOfModule {_%bool} _%bool _%bs.
+
+Definition tmMakeQuotationOfModuleAndRebase {debug:debug_opt} (do_existing_instance : bool) (reference_mp : qualid) (new_base_mp : modpath) : TemplateMonad _
+  := cs <- tmQuoteModule reference_mp;;
+     let cs := List.map (rebase_global_reference new_base_mp) cs in
+     tmMakeQuotationOfConstants do_existing_instance cs.
+Global Arguments tmMakeQuotationOfModuleAndRebase {_%bool} _%bool _%bs _.
 
 Module qKername <: QuotationOfOrderedType Kername.
   MetaCoq Run (tmMakeQuotationOfModule false "Kername").
   Module qOT <: QuotationOfOrderedTypeOrig Kername.OT.
-    Module M. Include Kername.OT. End M.
-    Goal True.
-
-      run_template_program (tmQuoteModule "M"%bs) (fun v => pose v).
-    MetaCoq Run (tmMakeQuotationOfModule false "Kername.OT").
-    Print Kername.OT
+    (* kludge around https://github.com/MetaCoq/metacoq/issues/847 *)
+    Module OT'. Include Kername.OT. End OT'.
+    MetaCoq Run (Kername_mp <- tmExtractBaseModPathFromMod "Kername";; tmMakeQuotationOfModuleAndRebase false "OT'" (MPdot Kername_mp "OT")).
   End qOT.
 End qKername.
+
 Module qKernameSet <: MSetAVL.QuotationOfMake Kername KernameSet.
-  MetaCoq Run (tmMakeQuotationOfModule false "KernameSet").
-End qKername.
-Fail Check KernameSetOrdProp.gtb.
-Module KernameSetOrdProp := MSetProperties.OrdProperties KernameSet.
+  (* kludge around https://github.com/MetaCoq/metacoq/issues/847 *)
+  Module KernameSet'. Include KernameSet. End KernameSet'.
+  Module qRaw.
+    Module Raw'. Include KernameSet.Raw. End Raw'.
+    MetaCoq Run (Kernames_mp <- tmExtractBaseModPathFromMod "Kernames";; tmMakeQuotationOfModuleAndRebase false "Raw'" (MPdot (MPdot Kernames_mp "KernameSet") "Raw")).
+  End qRaw.
+  MetaCoq Run (Kernames_mp <- tmExtractBaseModPathFromMod "Kernames";; tmMakeQuotationOfModuleAndRebase false "KernameSet'" (MPdot Kernames_mp "KernameSet")).
+End qKernameSet.
 Module qKernameSetOrdProp <: MSets.QuotationOfOrdProperties KernameSet KernameSetOrdProp qKername.
-  Module qME := QuotationOfOrderedTypeFacts KernameSet.E KernameSetOrdProp.ME qKernameSet.
+  Module qME := Structures.QuotationOfOrderedTypeFacts KernameSet.E KernameSetOrdProp.ME qKername.
   (*Module qML := QuotationOfOrderedTypeLists M.E F.ML.*)
   Module qP <: MSets.QuotationOfWProperties KernameSet KernameSetOrdProp.P.
-    MetaCoq Run (tmMakeQuotationOfModule false "KernameSetOrdProp.P").
+    Module qDec <: MSets.QuotationOfWDecideOn Kername KernameSet KernameSetOrdProp.P.Dec.
+      Module qF <: MSets.QuotationOfWFactsOn Kername KernameSet KernameSetOrdProp.P.Dec.F.
+        Module F'. Include KernameSetOrdProp.P.Dec.F. End F'.
+        MetaCoq Run (Kernames_mp <- tmExtractBaseModPathFromMod "Kernames";; tmMakeQuotationOfModuleAndRebase false "F'" (MPdot (MPdot (MPdot (MPdot Kernames_mp "KernameSetOrdProp") "P") "Dec") "F")).
+      End qF.
+      Module qMSetDecideAuxiliary.
+        Module MSetDecideAuxiliary'. Include KernameSetOrdProp.P.Dec.MSetDecideAuxiliary. End MSetDecideAuxiliary'.
+        MetaCoq Run (Kernames_mp <- tmExtractBaseModPathFromMod "Kernames";; tmMakeQuotationOfModuleAndRebase false "MSetDecideAuxiliary'" (MPdot (MPdot (MPdot (MPdot Kernames_mp "KernameSetOrdProp") "P") "Dec") "MSetDecideAuxiliary")).
+      End qMSetDecideAuxiliary.
+    End qDec.
+    Module qFM <: MSets.QuotationOfWFactsOn Kername KernameSet KernameSetOrdProp.P.FM.
+      Module FM'. Include KernameSetOrdProp.P.FM. End FM'.
+      MetaCoq Run (Kernames_mp <- tmExtractBaseModPathFromMod "Kernames";; tmMakeQuotationOfModuleAndRebase false "FM'" (MPdot (MPdot (MPdot Kernames_mp "KernameSetOrdProp") "P") "FM")).
+    End qFM.
+    Module P'. Include KernameSetOrdProp.P. End P'.
+    MetaCoq Run (Kernames_mp <- tmExtractBaseModPathFromMod "Kernames";; tmMakeQuotationOfModuleAndRebase false "P'" (MPdot (MPdot Kernames_mp "KernameSetOrdProp") "P")).
   End qP.
-  MetaCoq Run (tmMakeQuotationOfModule false "KernameSetOrdProp").
+  Module KernameSetOrdProp'. Include KernameSetOrdProp. End KernameSetOrdProp'.
+  MetaCoq Run (Kernames_mp <- tmExtractBaseModPathFromMod "Kernames";; tmMakeQuotationOfModuleAndRebase false "KernameSetOrdProp'" (MPdot Kernames_mp "KernameSetOrdProp")).
 End qKernameSetOrdProp.
 Module qKernameMap <: FMapAVL.QuotationOfMake Kername.OT KernameMap qKername.qOT.
   Module qRaw.
-    MetaCoq Run (tmMakeQuotationOfModule false "KernameMap.Raw").
+    Module Raw'. Include KernameMap.Raw. End Raw'.
+    MetaCoq Run (Kernames_mp <- tmExtractBaseModPathFromMod "Kernames";; tmMakeQuotationOfModuleAndRebase false "Raw'" (MPdot (MPdot Kernames_mp "KernameMap") "Raw")).
   End qRaw.
   MetaCoq Run (tmMakeQuotationOfModule false "KernameMap").
 End qKernameMap.
